mixfix/theorems/MixfixRepairConflictFree.v
@@ -1,0 +1,323 @@
+From disamb Require Export MixfixRepair.
+From disamb Require Import MyUtils.
+
+Section MixfixRepairConflictFree.
+
+Context {T : Type}.
+Implicit Types (t : parse_tree T) (ts : parse_forest T) (p : production T) (X : symbol T)
+  (g : mixfixgrammar T) (Xs : list (symbol T)) (b : bool) (Q : crules T).
+
+Lemma add_last_rncf Q p ts t :
+  (∀ p2, p CR p2 ∠ Q → p2 LM t → False) → rncf Q p (add_last ts t).
+Proof.
+  intros Hnlm p2 Hcr Hrn. induction ts; simpl in Hrn.
+  - inv Hrn.
+    inv H0.
+    eauto.
+    inv H1.
+  - inv Hrn.
+    inv H0.
+    destruct ts; inv H2.
+    apply IHts.
+    constructor. assumption.
+Qed.
+
+Lemma add_last_cff Q ts tn :
+  cff Q ts → cf Q tn → cff Q (add_last ts tn).
+Proof.
+  intros Hcff Hcf.
+  induction Hcff; simpl.
+  - constructor; auto. constructor.
+  - constructor; auto.
+Qed.
+
+Lemma repair_cr_forest_true_conflict Q p pn ts tns t' :
+  repair_cr_forest Q p pn ts tns = (t', true) → ∃ p2, p CR p2 ∠ Q ∧ (p2 = pn ∨ p2 LMf tns).
+Proof.
+  revert t' pn.
+  induction tns using parse_forest_tree_rec with
+    (P := fun tn => ∀ t', repair_cr Q p ts tn = (t', true) →
+                            ∃ p2, p CR p2 ∠ Q ∧ p2 LM tn); simpl.
+  - intros. inv H.
+  - rename p0 into pn.
+    intros. 
+    apply IHtns in H.
+    destruct H as [p2].
+    exists p2. destruct H.
+    split; auto.
+    destruct H0.
+    + subst.
+      constructor.
+    + constructor.
+      assumption.
+  - intros. inv H.
+  - rename p0 into tn.
+    intros.
+    destruct (repair_cr Q p ts tn) as [tn1' b] eqn:E.
+    destruct (decide (b = true ∨ p CR pn ∠ Q)).
+    + inv H.
+      destruct o.
+      * subst.
+        edestruct IHtns as [p2]; eauto.
+        destruct H.
+        exists p2.
+        split; auto.
+        right.
+        constructor.
+        assumption.
+      * exists pn.
+        split; auto.
+    + inv H.
+Qed.
+
+Lemma repair_cr_forest_conflict_true g X Q p p2 pn ts tns t' :
+  wft g X (node pn tns) →
+  p CR p2 ∠ Q →
+  (p2 = pn ∨ p2 LMf tns) →
+  ∃ t', repair_cr_forest Q p pn ts tns = (t', true).
+Proof.
+  intros.
+  inv H.
+  revert H1 H5 H6.
+  revert pn.
+  induction tns using parse_forest_tree_rec with
+    (P := fun tn => ∀ X, wft g X tn → p CR p2 ∠ Q → p2 LM tn → ∃ t', repair_cr Q p ts tn = (t', true)); simpl.
+  - intros.
+    inv H2.
+  - intros.
+    inv H.
+    apply IHtns in H7; auto.
+    inv H2; auto.
+  - intros.
+    exfalso.
+    inv H6.
+    destruct H1.
+    + subst.
+      apply conflict_right_well_formed in H0.
+      destruct H0.
+      inv H0.
+    + inv H.
+  - intros.
+    inv H6.
+    destruct (repair_cr Q p ts p0) eqn:E.
+    destruct (decide (b = true ∨ p CR X :: Xs ∠ Q)).
+    + eexists. eauto.
+    + exfalso.
+      apply IHtns in H4; auto. {
+        destruct H4.
+        inv H.
+        apply n.
+        auto.
+      } {
+        destruct H1.
+        - exfalso.
+          subst.
+          apply n.
+          auto.
+        - inv H.
+          assumption.
+      }
+Qed.
+
+Lemma add_last_lncf Q p ts tn1 tn2 :
+  ts ≠ nil_forest →
+  lncf Q p (add_last ts tn1) →
+  lncf Q p (add_last ts tn2).
+Proof.
+  intros ?????.
+  destruct ts; simpl in *.
+  - contradiction.
+  - inv H2.
+    eapply H0; eauto.
+    constructor.
+    assumption.
+Qed.
+
+Lemma add_last_rmf p ts tn :
+  p RMf add_last ts tn → p RM tn.
+Proof.
+  intro.
+  induction ts; simpl in H.
+  - inv H; auto.
+    inv H1.
+  - apply IHts.
+    inv H; auto.
+    destruct ts; inv H2.
+Qed.
+
+Lemma add_last_lm_rnf p ts tn :
+  p LM tn ↔ p RNf add_last ts tn.
+Proof.
+  split.
+  - intro.
+    induction ts; simpl.
+    + constructor.
+      assumption.
+    + constructor.
+      assumption.
+  - intro.
+    induction ts; simpl in H.
+    + inv H.
+      assumption.
+      inv H1.
+    + apply IHts.
+      inv H.
+      destruct ts; inv H2.
+      assumption.
+Qed.
+
+Lemma repair_cr_conflict_free g X Q p ts tn t' b :
+  safe_crules Q →
+  ts ≠ nil_forest →
+  wft g X tn →
+  lncf Q p (add_last ts tn) →
+  cff Q ts →
+  cf Q tn →
+  repair_cr Q p ts tn = (t', b) →
+  cf Q t'.
+Proof.
+  intro Hsafe. intros. revert H H0 H1 H2 H4. revert t' X b.
+  induction H3 using conflict_free_tree_forest
+    with (P0 := fun tns IHcfftns => ∀ X pn t' b,
+                                             ts ≠ nil_forest →
+                                             wft g X (node pn tns) →
+                                             cff Q ts →
+                                             lncf Q p (add_last ts (node pn tns)) →
+                                             lncf Q pn tns →
+                                             rncf Q pn tns →
+                                             repair_cr_forest Q p pn ts tns = (t', b) →
+                                             cf Q t').
+  - simpl.
+    intros.
+    inv H4.
+    constructor; auto.
+
+    apply add_last_rncf.
+    intros.
+    inv H4.
+
+    apply add_last_cff; auto.
+    constructor.
+  - rename p0 into pn, ts0 into tns.
+    simpl.
+    intros.
+    eapply IHconflict_free; eauto.
+  - simpl.
+    intros ????????? Hrncf ?.
+    inv H4.
+    constructor; auto.
+
+    apply add_last_rncf.
+    intros.
+    inv H5.
+    inv H0.
+    inv H9.
+    apply conflict_right_well_formed in H4. destruct H4.
+    inv H4.
+    inv H7.
+
+    apply add_last_cff; auto.
+    constructor.
+    intros ???. inv H5.
+    intros ???. inv H5. inv H7.
+    constructor.
+  - rename t into tn1, ts0 into tns.
+    intros ????????? Hrncf ?.
+    assert (Hrep := H5).
+    simpl in H5.
+    destruct (repair_cr Q p ts tn1) as [tns' bn] eqn:Hreptns1.
+    destruct (decide (bn = true ∨ p CR pn ∠ Q)).
+    + inv H5.
+      apply repair_cr_forest_true_conflict in Hrep.
+      destruct Hrep as [p2]. destruct H5.
+      inv H0.
+      inv H11.
+      apply IHconflict_free with (t' := tns') (b := bn) in H9 as ?; eauto using add_last_lncf.
+      constructor. {
+        intros p3 ??.
+        inv H8.
+        destruct tn1 as [a|pn1 tn1s]; simpl in Hreptns1.
+        - inv Hreptns1.
+          inv H13.
+          + destruct o.
+            inv H8.
+            eapply Hsafe; eauto.
+          + apply add_last_rmf in H11.
+            inv H11.
+        - destruct tn1s as [|tn11 tn1s]; simpl in Hreptns1.
+          + inv Hreptns1.
+            inv H13.
+            * destruct o.
+              inv H8.
+              eapply Hsafe; eauto.
+            * apply add_last_rmf in H11.
+              apply H4 with p3; auto.
+              constructor.
+              assumption.
+          + destruct (repair_cr Q p ts tn11) as [tn11' bn11] eqn:Hreptn11.
+            destruct (decide (bn11 = true ∨ p CR pn1 ∠ Q)).
+            * inv Hreptns1.
+              inv H13.
+              **apply H4 with pn1; auto.
+                constructor. constructor.
+              **apply H4 with p3; auto.
+                constructor. constructor.
+                inv H11.
+                ***exfalso.
+                  inv H9.
+                  inv H16.
+                  inv H17.
+                  inv H14.
+                  ****simpl in Hreptn11.
+                    inv Hreptn11.
+                    destruct o0.
+                    inv H8.
+                    apply conflict_right_well_formed in H8. destruct H8.
+                    inv H9.
+                  ****eapply acyclic_productions; eauto.
+                ***constructor.
+                  assumption.
+            * inv Hreptns1.
+              inv H13.
+              **destruct o.
+                inv H8.
+                eapply Hsafe; eauto.
+              **apply add_last_rmf in H11.
+                apply H4 with p3; auto.
+                constructor.
+                assumption.
+      } {
+        intros p3 ??.
+        inv H8.
+        inv H13.
+        - inv H12.
+          apply conflict_right_well_formed in H7. destruct H7.
+          inv H7.
+          eapply acyclic_productions; eauto.
+          inv H13.
+        - apply Hrncf with p3; auto.
+          constructor.
+          constructor.
+          assumption.
+      } {
+        constructor; auto.
+      }
+    + inv H5. constructor; auto. {
+        intros ???.
+        inv H6.
+        apply add_last_lm_rnf in H8.
+        eapply repair_cr_forest_conflict_true with (ts := ts) in H0; eauto. {
+          destruct H0.
+          rewrite Hrep in H0.
+          inv H0.
+        } {
+          inv H8; auto.
+        }
+      } {
+        apply add_last_cff; auto.
+        constructor; auto.
+        constructor; auto.
+      }
+Qed.
+
+End MixfixRepairConflictFree.
